test_congr.lean
@@ -1,0 +1,3 @@
+example (a b : Bool) (h : (a = true ↔ b = true)) : a = b := by
+  apply Bool.ext
+  exact h
